add impl for qinv

code/k256/Hacl.K256.Scalar.fst
@@ -18,9 +18,6 @@ module BD = Hacl.Bignum.Definitions
 module BN = Hacl.Bignum
 module BR = Hacl.Bignum.ModReduction
 module AM = Hacl.Bignum.AlmostMontgomery
-module BI = Hacl.Bignum.ModInv
-module BE = Hacl.Bignum.Exponentiation
-module BM = Hacl.Bignum.Montgomery
 module BB = Hacl.Bignum.Base
 
 module SN = Hacl.Spec.Bignum
@@ -232,19 +229,4 @@ let qmul out f1 f2 =
   SN.bn_mul_lemma (as_seq h0 f1) (as_seq h0 f2);
 
   modq out tmp;
-  pop_frame ()
-
-
-let qinv out f =
-  push_frame ();
-  let n = create qnlimb (u64 0) in
-  make_u64_4 n (make_order_k256 ());
-  let r2 = create 4ul (u64 0) in
-  make_u64_4 r2 (make_r2_modq ());
-  let mu = make_mu0 () in
-  let n2 = create qnlimb (u64 0) in
-  BI.bn_mod_inv_prime_n2 qnlimb n n2;
-
-  BE.bn_mod_exp_fw_vartime_precomp
-    (BM.mk_runtime_mont qnlimb) 4ul n mu r2 f 256ul n2 out;
   pop_frame ()
