code/k256/Hacl.Spec.K256.Qinv.fst
@@ -50,6 +50,72 @@ The algorithm is taken from
 https://briansmith.org/ecc-inversion-addition-chains-01
 *)
 
+val qinv_r0_r1 (x14: S.qelem) : S.qelem
+let qinv_r0_r1 x14 =
+  let x28 = S.qmul (qsquare_times x14 14) x14 in
+  let x56 = S.qmul (qsquare_times x28 28) x28 in
+  let r0 = S.qmul (qsquare_times x56 56) x56 in
+  let r1 = S.qmul (qsquare_times r0 14) x14 in
+  r1
+
+
+val qinv_r2_r8 (r1 x_101 x_111 x_1011: S.qelem) : S.qelem
+let qinv_r2_r8 r1 x_101 x_111 x_1011 =
+  let r2 = S.qmul (qsquare_times r1 3) x_101 in
+  let r3 = S.qmul (qsquare_times r2 4) x_111 in
+  let r4 = S.qmul (qsquare_times r3 4) x_101 in
+  let r5 = S.qmul (qsquare_times r4 5) x_1011 in
+  let r6 = S.qmul (qsquare_times r5 4) x_1011 in
+  let r7 = S.qmul (qsquare_times r6 4) x_111 in
+  let r8 = S.qmul (qsquare_times r7 5) x_111 in
+  r8
+
+
+val qinv_r9_r15 (r8 x_101 x_111 x_1001 x_1101: S.qelem) : S.qelem
+let qinv_r9_r15 r8 x_101 x_111 x_1001 x_1101 =
+  let r9 = S.qmul (qsquare_times r8 6) x_1101 in
+  let r10 = S.qmul (qsquare_times r9 4) x_101 in
+  let r11 = S.qmul (qsquare_times r10 3) x_111 in
+  let r12 = S.qmul (qsquare_times r11 5) x_1001 in
+  let r13 = S.qmul (qsquare_times r12 6) x_101 in
+  let r14 = S.qmul (qsquare_times r13 10) x_111 in
+  let r15 = S.qmul (qsquare_times r14 4) x_111 in
+  r15
+
+
+val qinv_r16_r23 (r15 x8 x_11 x_1001 x_1011 x_1101: S.qelem) : S.qelem
+let qinv_r16_r23 r15 x8 x_11 x_1001 x_1011 x_1101 =
+  let r16 = S.qmul (qsquare_times r15 9) x8 in
+  let r17 = S.qmul (qsquare_times r16 5) x_1001 in
+  let r18 = S.qmul (qsquare_times r17 6) x_1011 in
+  let r19 = S.qmul (qsquare_times r18 4) x_1101 in
+  let r20 = S.qmul (qsquare_times r19 5) x_11 in
+  let r21 = S.qmul (qsquare_times r20 6) x_1101 in
+  let r22 = S.qmul (qsquare_times r21 10) x_1101 in
+  let r23 = S.qmul (qsquare_times r22 4) x_1001 in
+  r23
+
+
+val qinv_r24_r25 (r23 x_1 x6: S.qelem) : S.qelem
+let qinv_r24_r25 r23 x_1 x6 =
+  let r24 = S.qmul (qsquare_times r23 6) x_1 in
+  let r25 = S.qmul (qsquare_times r24 8) x6 in
+  r25
+
+
+val qinv_r0_r25 (x_1 x_11 x_101 x_111 x_1001 x_1011 x_1101: S.qelem) : S.qelem
+let qinv_r0_r25 x_1 x_11 x_101 x_111 x_1001 x_1011 x_1101 =
+  let x6 = S.qmul (qsquare_times x_1101 2) x_1011 in
+  let x8 = S.qmul (qsquare_times x6 2) x_11 in
+  let x14 = S.qmul (qsquare_times x8 6) x6 in
+
+  let r1 = qinv_r0_r1 x14 in
+  let r8 = qinv_r2_r8 r1 x_101 x_111 x_1011 in
+  let r15 = qinv_r9_r15 r8 x_101 x_111 x_1001 x_1101 in
+  let r23 = qinv_r16_r23 r15 x8 x_11 x_1001 x_1011 x_1101 in
+  qinv_r24_r25 r23 x_1 x6
+
+
 val qinv: f:S.qelem -> S.qelem
 let qinv f =
   let x_1 = f in
@@ -61,39 +127,7 @@ let qinv f =
   let x_1011 = S.qmul x_10 x_1001 in
   let x_1101 = S.qmul x_10 x_1011 in
 
-  let x6 = S.qmul (qsquare_times x_1101 2) x_1011 in
-  let x8 = S.qmul (qsquare_times x6 2) x_11 in
-  let x14 = S.qmul (qsquare_times x8 6) x6 in
-  let x28 = S.qmul (qsquare_times x14 14) x14 in
-  let x56 = S.qmul (qsquare_times x28 28) x28 in
-
-  let r0 = S.qmul (qsquare_times x56 56) x56 in
-  let r1 = S.qmul (qsquare_times r0 14) x14 in
-  let r2 = S.qmul (qsquare_times r1 3) x_101 in
-  let r3 = S.qmul (qsquare_times r2 4) x_111 in
-  let r4 = S.qmul (qsquare_times r3 4) x_101 in
-  let r5 = S.qmul (qsquare_times r4 5) x_1011 in
-  let r6 = S.qmul (qsquare_times r5 4) x_1011 in
-  let r7 = S.qmul (qsquare_times r6 4) x_111 in
-  let r8 = S.qmul (qsquare_times r7 5) x_111 in
-  let r9 = S.qmul (qsquare_times r8 6) x_1101 in
-  let r10 = S.qmul (qsquare_times r9 4) x_101 in
-  let r11 = S.qmul (qsquare_times r10 3) x_111 in
-  let r12 = S.qmul (qsquare_times r11 5) x_1001 in
-  let r13 = S.qmul (qsquare_times r12 6) x_101 in
-  let r14 = S.qmul (qsquare_times r13 10) x_111 in
-  let r15 = S.qmul (qsquare_times r14 4) x_111 in
-  let r16 = S.qmul (qsquare_times r15 9) x8 in
-  let r17 = S.qmul (qsquare_times r16 5) x_1001 in
-  let r18 = S.qmul (qsquare_times r17 6) x_1011 in
-  let r19 = S.qmul (qsquare_times r18 4) x_1101 in
-  let r20 = S.qmul (qsquare_times r19 5) x_11 in
-  let r21 = S.qmul (qsquare_times r20 6) x_1101 in
-  let r22 = S.qmul (qsquare_times r21 10) x_1101 in
-  let r23 = S.qmul (qsquare_times r22 4) x_1001 in
-  let r24 = S.qmul (qsquare_times r23 6) x_1 in
-  let r25 = S.qmul (qsquare_times r24 8) x6 in
-  r25
+  qinv_r0_r25 x_1 x_11 x_101 x_111 x_1001 x_1011 x_1101
 
 
 val lemma_pow_mod_1: f:S.qelem -> Lemma (f == M.pow f 1 % S.q)
@@ -335,3 +369,10 @@ let qinv_lemma f =
   assert_norm (pow2 8 = 0x100);
   lemma_pow_pow_mod_mul f 0xfffffffffffffffffffffffffffffffebaaedce6af48a03bbfd25e8cd03641 0x100 0x3f;
   assert (r25 == M.pow f 0xfffffffffffffffffffffffffffffffebaaedce6af48a03bbfd25e8cd036413f % S.q)
+
+
+val qinv_is_qinv_lemma: f:S.qelem -> Lemma (qinv f == S.qinv f)
+let qinv_is_qinv_lemma f =
+  qinv_lemma f;
+  assert (qinv f == M.pow f (S.q - 2) % S.q);
+  M.lemma_pow_mod #S.q f (S.q - 2)
