code/k256/Hacl.K256.Scalar.fsti
@@ -135,12 +135,3 @@ val qmul (out f1 f2: qelem) : Stack unit
   (ensures  fun h0 _ h1 -> modifies (loc out) h0 h1 /\
     qas_nat h1 out == S.qmul (qas_nat h0 f1) (qas_nat h0 f2) /\
     qe_lt_q h1 out)
-
-
-val qinv (out f: qelem) : Stack unit
-  (requires fun h ->
-    live h out /\ live h f /\ disjoint out f /\
-    qe_lt_q h f)
-  (ensures  fun h0 _ h1 -> modifies (loc out) h0 h1 /\
-    qas_nat h1 out == S.qinv (qas_nat h0 f)  /\
-    qe_lt_q h1 out)
